theories/Term.v
@@ -20,359 +20,267 @@ Implicit Type t: type.
 Implicit Type N: normal.
 Implicit Types x y: var.
 
-Module ProofTree.
-  Inductive Jv: Set :=
-  | Jv_var Γ x
-  | Jv_tt Γ
-  | Jv_fanout: Jv → Jv → Jv
-  | Jv_fst: Jv → Jv
-  | Jv_snd: Jv → Jv.
-
-  Function envof (v: Jv): environment :=
-    match v with
-    | Jv_var Γ _ => Γ
-    | Jv_tt Γ => Γ
-    | Jv_fanout p1 _ => envof p1
-    | Jv_fst p => envof p
-    | Jv_snd p => envof p
-    end.
-
-  Function termof (v: Jv): term :=
-    match v with
-    | Jv_var _ x => v_var x
-    | Jv_tt _ => v_tt
-    | Jv_fst p => v_fst (termof p)
-    | Jv_snd p => v_snd (termof p)
-    | Jv_fanout p1 p2 => v_fanout (termof p1) (termof p2)
-    end.
-
-  #[local]
-  Definition unknown_type := opaque (λ _: Jv, t_unit).
-
-
-  Function typeof (v: Jv): type :=
-    match v with
-    | Jv_var Γ x => if find x Γ is Some t then t else unknown_type v
-    | Jv_tt _ => t_unit
-    | Jv_fst p => if typeof p is t * _ then t else unknown_type v
-    | Jv_snd p => if typeof p is _ * t then t else unknown_type v
-    | Jv_fanout p1 p2 => typeof p1 * typeof p2
-    end.
-
-  Definition asserts (v: Jv): Prop := envof v ⊢ termof v in typeof v.
-
-  Notation "'test' p" := (match p with | left _ => true | right _ => false end) (at level 1).
-
-  Function check (p: Jv): bool :=
-    match p with
-    | Jv_var Γ x =>
-        if find x Γ is Some t then true else false
-    | Jv_tt _ => true
-    | Jv_fst p =>
-        (if typeof p is _ * _ then true else false)
-        && check p
-    | Jv_snd p =>
-        (if typeof p is _ * _ then true else false)
-        && check p
-    | Jv_fanout p1 p2 =>
-        test (eq_environment (envof p1) (envof p2))
-        && check p1
-        && check p2
-    end %bool.
-
-  Lemma check_sound (p: Jv): Bool.Is_true (check p) → asserts p.
-  Proof.
-    unfold asserts.
-    functional induction (check p).
-    all: cbn.
-    all: intro q.
-    all: try contradiction.
-    - rewrite e0.
-      constructor.
-      apply Environment.find_sound.
-      auto.
-    - constructor.
-    - rewrite e0.
-      rewrite e0 in IHb.
-      destruct (check p0).
-      2: contradiction.
-      econstructor.
-      eauto.
-    - rewrite e0.
-      rewrite e0 in IHb.
-      destruct (check p0).
-      2: contradiction.
-      econstructor.
-      eauto.
-    - rewrite <- _x in IHb0.
-      destruct (check p1).
-      2: contradiction.
-      destruct (check p2).
-      2: contradiction.
-      constructor.
-      all: auto.
-  Qed.
-
-  Lemma check_complete {Γ v t}:
-    Γ ⊢ v in t →
-             ∃ p,
-               Γ = envof p ∧
-               v = termof p ∧
-               t = typeof p ∧
-               Bool.Is_true (check p).
-  Proof.
-    intro q.
-    induction q.
-    all: cbn.
-    - exists (Jv_var Γ x).
-      cbn.
-      rewrite (find_complete H).
-      all: repeat split; auto.
-    - exists (Jv_tt Γ).
-      cbn.
-      all: repeat split; auto.
-    - destruct IHq1 as [p1 [? [? []]]].
-      destruct IHq2 as [p2 [? [? []]]].
-      subst.
-      exists (Jv_fanout p1 p2).
-      cbn.
-      destruct (check p1).
-      2: contradiction.
-      destruct (check p2).
-      2: contradiction.
-      rewrite H3.
-      all: repeat split; auto.
-      destruct eq_environment.
-      2: contradiction.
-      cbn.
-      auto.
-    - destruct IHq as [p1 [? [? []]]].
-      subst.
-      exists (Jv_fst p1).
-      cbn.
-      rewrite <- H1.
-      destruct (check p1).
-      2: contradiction.
-      all: repeat split; auto.
-    - destruct IHq as [p1 [? [? []]]].
-      subst.
-      exists (Jv_snd p1).
-      cbn.
-      rewrite <- H1.
-      destruct (check p1).
-      2: contradiction.
-      all: repeat split; auto.
-  Qed.
-
-  Function elaborate Γ v: option Jv :=
-    match v with
-    | v_var x =>
-        do _ ← find x Γ ;
-        Some (Jv_var Γ x)
-    | v_tt => Some (Jv_tt Γ)
-    | v_fst v =>
-        do p ← elaborate Γ v ;
-        if typeof p is _ * _
-        then
-          Some (Jv_fst p)
-        else
-          None
-    | v_snd v =>
-        do p ← elaborate Γ v ;
-        if typeof p is _ * _
-        then
-          Some (Jv_snd p)
-        else
-          None
-    | v_fanout v0 v1 =>
-        do v0' ← elaborate Γ v0 ;
-        do v1' ← elaborate Γ v1 ;
-        Some (Jv_fanout v0' v1')
-    end.
-
-  Lemma termof_elaborate {Γ v p}: elaborate Γ v = Some p → termof p = v.
-  Proof.
-    generalize dependent p.
-    functional induction (elaborate Γ v).
-    all: intros ? q.
-    all: inversion q.
-    all: subst.
-    all: cbn.
-    all: auto.
-    - rewrite IHo.
-      all: auto.
-    - rewrite IHo.
-      all: auto.
-    - rewrite IHo, IHo0.
-      all: auto.
-  Qed.
-
-  Lemma envof_elaborate {Γ v p}: elaborate Γ v = Some p → envof p = Γ.
-  Proof.
-    generalize dependent p.
-    functional induction (elaborate Γ v).
-    all: intros ? q.
-    all: inversion q.
-    all: subst.
-    all: cbn.
-    all: auto.
-  Qed.
-
-  Definition elaborate_sound {Γ v p}:
-    elaborate Γ v = Some p → Bool.Is_true (check p).
-  Proof.
-    generalize dependent p.
-    functional induction (elaborate Γ v).
-    all: cbn.
-    all: intros ? q.
-    all: inversion q.
-    all: subst.
-    - cbn.
-      rewrite e0.
-      cbv.
-      auto.
-    - cbn.
-      auto.
-    - cbn.
-      rewrite e1.
-      cbn.
-      assert (IHo' := IHo _ e0).
-      auto.
-    - cbn.
-      rewrite e1.
-      cbn.
-      assert (IHo' := IHo _ e0).
-      auto.
-    - cbn.
-      assert (IHo' := IHo _ e0).
-      assert (IHo0' := IHo0 _ e1).
-      rewrite (envof_elaborate e0).
-      rewrite (envof_elaborate e1).
-      destruct eq_environment.
-      2: contradiction.
-      cbn.
-      destruct (check v0').
-      2: contradiction.
-      destruct (check v1').
-      2: contradiction.
-      auto.
-  Qed.
-End ProofTree.
-
-Function typecheck Γ v :=
-  match v with
-  | v_var x => find x Γ
-  | v_tt => Some t_unit
-  | v_fst v =>
-      do t0 * _ ← typecheck Γ v ;
+Function typecheck Γ v t: bool :=
+  match v, t with
+  | v_tt, t_unit => true
+  | v_fanout v0 v1, t1 * t2 =>
+      typecheck Γ v0 t1 && typecheck Γ v1 t2
+  | v_neu v, _ =>
+      if typeinfer Γ v is Some t'
+      then if eq_type t t' then true else false
+      else false
+  | _, _ => false
+  end %bool
+with typeinfer Γ V :=
+  match V with
+  | V_var x => find x Γ
+  | V_fst V =>
+      do t0 * _ ← typeinfer Γ V ;
       Some t0
-  | v_snd v =>
-      do _ * t1 ← typecheck Γ v ;
+  | V_snd V =>
+      do _ * t1 ← typeinfer Γ V ;
       Some t1
-  | v_fanout v0 v1 =>
-      do t0 ← typecheck Γ v0 ;
-      do t1 ← typecheck Γ v1 ;
-      Some (t0 * t1)
+  | V_cut v t =>
+      if typecheck Γ v t
+      then Some t
+      else None
   end.
 
-Function eval v :=
+Function intro v :=
   match v with
-  | v_var _ => None
   | v_tt => Some N_tt
-  | v_fst v =>
-      do N_fanout a _ ← eval v ;
-      Some a
-  | v_snd v =>
-      do N_fanout _ a ← eval v ;
-      Some a
   | v_fanout v0 v1 =>
-      do v0' ← eval v0 ;
-      do v1' ← eval v1 ;
+      do v0' ← intro v0 ;
+      do v1' ← intro v1 ;
       Some (N_fanout v0' v1')
+  | v_neu V => elim V
+  end
+with elim (V: expr) :=
+  match V with
+  | V_var _ => None
+  | V_fst V =>
+      do N_fanout a _ ← elim V ;
+      Some a
+  | V_snd V =>
+      do N_fanout _ a ← elim V ;
+      Some a
+  | V_cut v _ => intro v
   end.
 
 Theorem typecheck_sound:
-  ∀ {Γ v t}, typecheck Γ v = Some t → Γ ⊢ v in t.
+  ∀ {Γ v t}, Bool.Is_true (typecheck Γ v t) → Γ ⊢ v in t
+with typeinfer_sound:
+  ∀ {Γ V t}, typeinfer Γ V = Some t → JV Γ V t.
 Proof using .
-  intros Γ v.
-  functional induction (typecheck Γ v).
-  all: cbn.
-  all: intros ? p.
-  all: inversion p.
-  all: subst.
-  all: econstructor.
-  all: eauto.
-  apply find_sound.
-  auto.
+  - intros Γ v t p.
+    destruct v.
+    all: cbn.
+    + destruct t.
+      2: contradiction.
+      constructor.
+    + destruct t.
+      1: contradiction.
+      cbn in p.
+      destruct typecheck eqn:q1.
+      2: contradiction.
+      destruct typecheck eqn:q2 in p.
+      2: contradiction.
+      constructor.
+      * apply typecheck_sound.
+        rewrite q1.
+        apply I.
+      * apply typecheck_sound.
+        rewrite q2.
+        apply I.
+    + cbn in p.
+      constructor.
+      apply typeinfer_sound.
+      destruct typeinfer.
+      2: contradiction.
+      destruct eq_type.
+      2: contradiction.
+      subst.
+      auto.
+  - intros Γ V t p.
+    destruct V.
+    all: cbn.
+    + cbn in p.
+      constructor.
+      apply find_sound.
+      auto.
+    + cbn in p.
+      destruct typeinfer eqn:q.
+      2: discriminate.
+      destruct t0.
+      1: discriminate.
+      inversion p.
+      subst.
+      econstructor.
+      apply typeinfer_sound.
+      eauto.
+    + cbn in p.
+      destruct typeinfer eqn:q.
+      2: discriminate.
+      destruct t0.
+      1: discriminate.
+      inversion p.
+      subst.
+      econstructor.
+      apply typeinfer_sound.
+      eauto.
+    + cbn in p.
+      destruct typecheck eqn:q.
+      2: discriminate.
+      inversion p.
+      subst.
+      constructor.
+      apply typecheck_sound.
+      rewrite q.
+      apply I.
 Qed.
 
 Theorem typecheck_complete:
-  ∀ {Γ v t}, Γ ⊢ v in t → typecheck Γ v = Some t.
+  ∀ {Γ v t}, Γ ⊢ v in t → typecheck Γ v t = true
+with typeinfer_complete:
+  ∀ {Γ V t}, JV Γ V t → typeinfer Γ V = Some t.
 Proof using .
-  intros Γ ? ? p.
-  induction p.
-  all: cbn.
-  all: cbn in *.
-  all: try (destruct (typecheck Γ v) as [[]|]).
-  all: try (destruct (typecheck Γ v1)).
-  all: try (destruct (typecheck Γ v2)).
-  all: auto.
-  all: try inversion IHp.
-  all: subst.
-  all: try inversion IHp1.
-  all: subst.
-  all: try inversion IHp2.
-  all: subst.
-  all: auto.
-  apply find_complete.
-  auto.
+  - intros Γ ? ? p.
+    destruct p.
+    all: cbn in *.
+    all: auto.
+    all: try rewrite typecheck_complete.
+    all: try rewrite typecheck_complete.
+    all: auto.
+    rewrite (typeinfer_complete Γ V t).
+    2: auto.
+    destruct eq_type.
+    2: contradiction.
+    auto.
+  - intros Γ ? ? p.
+    destruct p.
+    all: cbn in *.
+    + apply find_complete.
+      auto.
+    + rewrite (typeinfer_complete Γ V _ p).
+      auto.
+    + rewrite (typeinfer_complete Γ V _ p).
+      auto.
+    + rewrite typecheck_complete.
+      all: auto.
 Qed.
 
-Theorem eval_sound:
-  ∀ {v N}, eval v = Some N → v ⇓ N.
+Theorem intro_sound:
+  ∀ {v N}, intro v = Some N → v ⇓ N
+with elim_sound:
+  ∀ {V N}, elim V = Some N → bigV V N
+.
 Proof using.
-  intros v.
-  functional induction (eval v).
-  all: intros ? p.
-  all: inversion p.
-  all: subst.
-  all: econstructor.
-  all: eauto.
+  - intros v N p.
+    destruct v.
+    all: cbn in p.
+    + inversion p.
+      constructor.
+    + destruct intro eqn:q1.
+      2: discriminate.
+      destruct intro eqn:q2 in p.
+      2: discriminate.
+      inversion p.
+      constructor.
+      all: auto.
+    + constructor.
+      apply elim_sound.
+      auto.
+  - intros V N p.
+    destruct V.
+    all: cbn in p.
+    + inversion p.
+    + destruct elim eqn:q1.
+      2: discriminate.
+      destruct n.
+      1: discriminate.
+      inversion p.
+      subst.
+      econstructor.
+      eauto.
+    + destruct elim eqn:q1.
+      2: discriminate.
+      destruct n.
+      1: discriminate.
+      inversion p.
+      subst.
+      econstructor.
+      eauto.
+    + constructor.
+      apply intro_sound.
+      auto.
 Qed.
 
-Theorem eval_complete:
-  ∀ {v N}, v ⇓ N → eval v = Some N.
+Theorem intro_complete:
+  ∀ {v N}, v ⇓ N → intro v = Some N
+with
+elim_complete:
+  ∀ {V N},
+       bigV V N → elim V = Some N.
 Proof using.
-  intros ? ? p.
-  induction p.
-  all: cbn.
-  all: try rewrite IHp.
-  all: try rewrite IHp1.
-  all: try rewrite IHp2.
-  all: reflexivity.
+  - intros ? ? p.
+    destruct p.
+    all: cbn.
+    + auto.
+    + repeat erewrite intro_complete.
+      all: eauto.
+    + auto.
+  - intros ? ? p.
+    destruct p.
+    all: cbn.
+    + repeat erewrite elim_complete.
+      all: eauto.
+      cbn.
+      auto.
+    + repeat erewrite elim_complete.
+      all: eauto.
+      cbn.
+      auto.
+    + apply intro_complete.
+      auto.
 Qed.
 
-Theorem big_preserve:
+Theorem intro_preserve:
   ∀ {v N},
     v ⇓ N →
-    ∀ Γ t, Γ ⊢ v in t → Γ ⊢ N in t.
+    ∀ Γ t, Γ ⊢ v in t → Γ ⊢ N in t
+with elim_preserve:
+  ∀ {V N},
+    bigV V N →
+    ∀ Γ t, JV Γ V t → Γ ⊢ N in t
+.
 Proof using.
-  intros v v' p.
-  induction p.
-  all: intros ? ? q.
-  all: inversion q.
-  all: subst.
-  all: auto.
-  - econstructor.
-    all: eauto.
-  - set (p' := IHp _ _ H1).
-    inversion p'.
-    subst.
-    auto.
-  - set (p' := IHp _ _ H1).
-    inversion p'.
-    subst.
-    auto.
+  - intros v N p.
+    destruct p.
+    all: intros ? ? q.
+    all: inversion q.
+    all: subst.
+    all: cbn.
+    + auto.
+    + constructor.
+      all: eauto.
+    + eapply elim_preserve.
+      all: eauto.
+  - intros V N p.
+    destruct p.
+    all: intros ? ? q.
+    all: inversion q.
+    all: subst.
+    all: cbn.
+    + assert (H1' := elim_preserve _ _ p _ _ H1).
+      cbn in H1'.
+      inversion H1'.
+      auto.
+    + assert (H1' := elim_preserve _ _ p _ _ H1).
+      cbn in H1'.
+      inversion H1'.
+      auto.
+    + eapply intro_preserve.
+      all: eauto.
 Qed.
 
 Theorem big_unique:
@@ -380,49 +288,62 @@ Theorem big_unique:
     v ⇓ N → v ⇓ N' → N = N'.
 Proof using.
   intros v N N' p q.
-  set (p' := eval_complete p).
-  set (q' := eval_complete q).
+  set (p' := intro_complete p).
+  set (q' := intro_complete q).
   rewrite p' in q'.
   inversion q'.
   auto.
 Qed.
 
-Theorem normalize:
+Theorem intro_normal:
   ∀ {v t},
    nil ⊢ v in t →
-   ∃ N, v ⇓ N.
+   ∃ N, v ⇓ N
+with elim_normal:
+  ∀ {V t},
+   JV nil V t →
+   ∃ N, bigV V N.
 Proof using.
-  intros v.
-  induction v.
-  all: intros ? p.
-  all: inversion p.
-  all: subst.
-  - inversion H1.
-  - exists N_tt.
-    constructor.
-  - destruct (IHv _ H1) as [v' s].
-    set (vwf := big_preserve s _ _ H1).
-    destruct v'.
-    all: cbn in *.
-    all: inversion vwf.
-    subst.
-    exists v'1.
-    econstructor.
-    eauto.
-  - destruct (IHv _ H1) as [v' s].
-    set (vwf := big_preserve s _ _ H1).
-    destruct v'.
-    all: cbn in *.
-    all: inversion vwf.
-    subst.
-    exists v'2.
-    econstructor.
-    eauto.
-  - destruct (IHv1 _ H2) as [v1' s1].
-    destruct (IHv2 _ H4) as [v2' s2].
-    exists (N_fanout v1' v2').
-    constructor.
-    all: auto.
+  - intros v t p.
+    destruct v.
+    all: inversion p.
+    all: subst.
+    + exists N_tt.
+      constructor.
+    + destruct (intro_normal _ _ H2) as [N1 s1].
+      destruct (intro_normal _ _ H4) as [N2 s2].
+      exists (N_fanout N1 N2).
+      constructor.
+      all: auto.
+    + destruct (elim_normal _ _ H1) as [N s].
+      exists N.
+      constructor.
+      auto.
+  - intros V t p.
+    destruct V.
+    all: inversion p.
+    all: subst.
+    + inversion H1.
+    + destruct (elim_normal _ _ H1) as [N s].
+      assert (wf := elim_preserve s _ _ H1).
+      destruct N.
+      all: inversion wf.
+      subst.
+      exists N1.
+      econstructor.
+      eauto.
+    + destruct (elim_normal _ _ H1) as [N s].
+      assert (wf := elim_preserve s _ _ H1).
+      destruct N.
+      all: inversion wf.
+      subst.
+      exists N2.
+      econstructor.
+      eauto.
+    + destruct (intro_normal _ _ H3) as [N s].
+      exists N.
+      constructor.
+      auto.
 Qed.
 
 Lemma big_normal:
@@ -438,22 +359,32 @@ Qed.
 Definition oftype Γ A := { v | Γ ⊢ v in A }.
 
 Lemma subst_var {x v}:
-  subst_term (v_var x) x v = v.
+  subst_term (V_var x) x v = v
+with
+  subst_var_elim {x V}:
+  subst_expr (V_var x) x V = V.
 Proof.
-  induction v.
-  all: cbn.
-  all: auto.
-  - destruct (eq_var x0 x).
+  - destruct v.
+    all: cbn.
     all: auto.
-  - rewrite IHv.
-    auto.
-  - rewrite IHv.
-    auto.
-  - rewrite IHv1, IHv2.
-    auto.
+    + repeat rewrite subst_var.
+      auto.
+    + rewrite subst_var_elim.
+      auto.
+  - destruct V.
+    all: cbn.
+    all: auto.
+    + destruct (eq_var x0 x).
+      all: auto.
+    + rewrite subst_var_elim.
+      auto.
+    + rewrite subst_var_elim.
+      auto.
+    + rewrite subst_var.
+      auto.
 Qed.
 
-Lemma subst_normal {v x N}: subst_term v x N = N.
+Lemma subst_normal {V x N}: subst_term V x N = N.
 Proof using.
   induction N.
   1: reflexivity.
@@ -462,467 +393,45 @@ Proof using.
   reflexivity.
 Qed.
 
-Lemma subst_preserve_minus:
-  ∀ {Γ v' t x},
-    minus x Γ ⊢ v' in t →
-  ∀ {v t'},
-    find x Γ = Some t →
-    Γ ⊢ v in t' →
-    minus x Γ ⊢ subst_term v' x v in t'.
-Proof using.
-  intros Γ v' t x p v.
-  induction v.
-  all: cbn.
-  all: intros t' ? q.
-  all: inversion q.
-  all: subst.
-  all: try (econstructor; eauto).
-  clear q.
-  assert (H2' := find_complete H2).
-  clear H2.
-  destruct eq_var.
-  - subst.
-    rewrite H in H2'.
-    inversion H2'.
-    subst.
-    auto.
-  - clear p H.
-    constructor.
-    apply find_sound.
-    rewrite find_minus.
-    all: auto.
-Qed.
-
-Lemma subst_preserve:
-  ∀ {Γ v' t x},
-    Γ ⊢ v' in t →
+Lemma
+  subst_preserve:
+  ∀ {Γ V' t x},
+    JV Γ V' t →
   ∀ {v t'},
     cons (x, t) Γ ⊢ v in t' →
-    Γ ⊢ subst_term v' x v in t'.
+                         Γ ⊢ subst_term V' x v in t'
+with
+  subst_preserve_elim:
+  ∀ {Γ V' t x},
+    JV Γ V' t →
+  ∀ {V t'},
+    JV (cons (x, t) Γ) V t' →
+    JV Γ (subst_expr V' x V) t'
+.
 Proof using.
-  intros Γ v' t x p v.
-  induction v.
-  all: cbn.
-  all: intros t' q.
-  all: inversion q.
-  all: subst.
-  all: try (econstructor; eauto).
-  destruct eq_var.
-  - subst.
-    inversion H1.
-    2: contradiction.
-    subst.
-    auto.
-  - inversion H1.
-    1: contradiction.
-    subst.
-    constructor.
-    auto.
-Qed.
-
-Lemma subst_assoc {x f g h}:
-  subst_term (subst_term h x g) x f = subst_term h x (subst_term g x f).
-Proof.
-  induction f.
-  all: cbn.
-  all: auto.
-  - destruct eq_var eqn:q.
-    1: auto.
-    cbn.
-    rewrite q.
-    auto.
-  - rewrite IHf.
-    auto.
-  - rewrite IHf.
-    auto.
-  - rewrite IHf1.
-    rewrite IHf2.
-    auto.
-Qed.
-
-Lemma msubst_normal {p N}: msubst p N = N.
-Proof using.
-  induction p.
-  1: reflexivity.
-  cbn.
-  destruct a.
-  rewrite subst_normal.
-  auto.
-Qed.
-
-Lemma msubst_preserve:
-  ∀ {p Γ v t},
-    Jp p Γ →
-    Γ ⊢ v in t →
-    nil ⊢ msubst p v in t.
-Proof using.
-  intros p.
-  induction p.
-  all: cbn.
-  all: intros.
-  - inversion H.
-    subst.
-    auto.
-  - destruct a.
-    inversion H.
-    subst.
-    eapply IHp.
-    2: eapply subst_preserve.
-    all: eauto.
-Qed.
-
-Lemma msubst_fst {p}:
-  ∀ {v}, msubst p (v_fst v) = v_fst (msubst p v).
-Proof.
-  induction p.
-  all: cbn.
-  1: auto.
-  destruct a.
-  intro.
-  rewrite IHp.
-  reflexivity.
-Qed.
-
-Lemma msubst_snd {p}:
-  ∀ {v}, msubst p (v_snd v) = v_snd (msubst p v).
-Proof.
-  induction p.
-  all: cbn.
-  1: auto.
-  destruct a.
-  intro.
-  rewrite IHp.
-  reflexivity.
-Qed.
-
-Lemma msubst_fanout {p}:
-  ∀ {v v'}, msubst p (v_fanout v v') = v_fanout (msubst p v) (msubst p v').
-Proof.
-  induction p.
-  all: cbn.
-  1: auto.
-  destruct a.
-  intros.
-  rewrite IHp.
-  reflexivity.
-Qed.
-
-Definition equiv {Γ t}: Relation_Definitions.relation (oftype Γ t) :=
-  λ o o',
-  ∀ p,
-    Jp p Γ →
-    ∃ N, (msubst p (proj1_sig o) ⇓ N) ∧ (msubst p (proj1_sig o') ⇓ N).
-
-Instance equiv_Reflexive Γ t: Reflexive (@equiv Γ t).
-Proof using.
-  unfold equiv.
-  intros [v p].
-  cbn.
-  intros σ ?.
-  destruct (@normalize (msubst σ v) t).
-  - eapply msubst_preserve.
-    all: eauto.
-  - exists x.
-    split.
-    all: auto.
-Qed.
-
-Instance equiv_Symmetric Γ t: Symmetric (@equiv Γ t).
-Proof using.
-  unfold equiv.
-  intros [v p] [v' q].
-  cbn.
-  intros f σ r.
-  destruct (f σ r).
-  destruct H.
-  exists x.
-  split.
-  all: auto.
-Qed.
-
-Instance equiv_Transitive Γ t: Transitive (@equiv Γ t).
-Proof using.
-  unfold equiv.
-  intros [x p] [y q] [z r].
-  cbn.
-  intros f g σ u.
-  destruct (f σ u), (g σ u).
-  destruct H, H0.
-  set (q' := big_unique H1 H0).
-  repeat rewrite q' in *.
-  exists x1.
-  split.
-  all: auto.
-Qed.
-
-Instance equiv_Equivalence Γ t: Equivalence (@equiv Γ t) := {
-    Equivalence_Reflexive := _ ;
-}.
-
-Instance oftype_Setoid Γ t: Setoid (oftype Γ t) := {
-    equiv := equiv ;
-}.
-
-Lemma map:
-  ∀ {v t Γ Δ},
-    (∀ x t, mem x t Γ → mem x t Δ) →
-    Γ ⊢ v in t →
-    Δ ⊢ v in t.
-Proof.
-  intro v.
-  induction v.
-  all: intros ? ? ? ? p.
-  all: inversion p.
-  all: subst.
-  all: try econstructor.
-  all: eauto.
-Qed.
-
-Definition linmap Γ Γ' := ∀ v t, Γ ⊢ v in t → Γ' ⊢ v in t.
-
-Lemma map_mem {Γ Γ'}:
-  linmap Γ Γ' →
-  ∀ {x t}, mem x t Γ → mem x t Γ'.
-Proof.
-  unfold linmap.
-  intros p.
-  intros x t q.
-  assert (q' := p _ _ (Jv_var _ _ _ q)).
-  inversion q'.
-  subst.
-  auto.
-Qed.
-
-Definition shadow {v Γ x t0 t1 t2}:
-  ((x, t0) :: Γ) ⊢ v in t2 → ((x, t0) :: (x, t1) :: Γ) ⊢ v in t2 :=
-  map Environment.shadow.
-
-Definition unshadow {v Γ x t0 t1 t2}:
-  (x, t0) :: (x, t1) :: Γ ⊢ v in t2 → (x, t0) :: Γ ⊢ v in t2 :=
-  map Environment.unshadow.
-
-Module Dec.
-  Inductive term {Γ: environment}: type → Set :=
-  | v_var {t} (x: var): find x Γ = Some t → term t
-  | v_tt: term t_unit
-  | v_fst {t t'} (v: term (t * t')): term t
-  | v_snd {t t'} (v: term (t * t')): term t'
-  | v_fanout {t t'} (v: term t) (v': term t'): term (t * t').
-  Arguments term: clear implicits.
-
-  Import OptionNotations.
-
-  Definition find_dec x Γ: option {t | find x Γ = Some t}.
-  Proof.
-    destruct (find x Γ).
-    2: apply None.
-    apply Some.
-    exists t.
-    auto.
-  Defined.
-
-  Fixpoint dec' Γ v: option { t & term Γ t } :=
-    match v with
-    | Spec.v_var x =>
-        match find_dec x Γ with
-        | Some p =>
-            Some (existT (term Γ) (proj1_sig p) (@v_var _ (proj1_sig p) x (proj2_sig p)))
-        | _ => None
-        end
-    | Spec.v_tt => Some (existT  (term Γ) t_unit v_tt)
-    | Spec.v_fst v =>
-        do existT _ (t0 * t1) v' ← dec' Γ v ;
-        Some (existT _ t0 (v_fst v'))
-    | Spec.v_snd v =>
-        do existT _ (t0 * t1) v' ← dec' Γ v ;
-        Some (existT (term Γ) t1 (v_snd v'))
-    | Spec.v_fanout v v' =>
-        do existT _ t0 v0 ← dec' Γ v ;
-        do existT _ t1 v1 ← dec' Γ v' ;
-        Some (existT (term Γ) (t0 * t1) (v_fanout v0 v1))
-    end.
-
-  Lemma dec_sound {Γ} v:
-    typecheck Γ v = (do d ← dec' Γ v ;
-                     Some (projT1 d)).
-  Proof.
-    induction v.
+  - intros Γ V' t x p v.
+    destruct v.
     all: cbn.
-    all: auto.
-    - destruct (find_dec x Γ) eqn:q.
-      + cbn.
-        destruct s.
-        cbn.
-        auto.
-      + cbn.
-        unfold find_dec in q.
-        destruct (find x Γ).
-        * discriminate.
-        * auto.
-    - rewrite IHv.
-      destruct (dec' Γ v).
-      2: auto.
-      destruct s.
-      cbn.
-      destruct x.
-      all: auto.
-    - rewrite IHv.
-      destruct (dec' Γ v).
-      2: auto.
-      destruct s.
-      cbn.
-      destruct x.
-      all: auto.
-    - rewrite IHv1.
-      rewrite IHv2.
-      destruct (dec' Γ v1).
-      2: auto.
-      destruct s.
-      destruct (dec' Γ v2).
-      2: auto.
-      destruct s.
-      cbn.
-      auto.
-  Defined.
-
-  Definition dec {Γ} t v (p: typecheck Γ v = Some t): term Γ t.
-  Proof.
-    rewrite dec_sound in p.
-    destruct (dec' Γ v).
-    2: discriminate.
-    destruct s.
-    cbn in p.
-    inversion p.
-    subst.
-    apply t0.
-  Defined.
-
-  Fixpoint undec {Γ t} (v: term Γ t) :=
-    match v with
-    | v_var x _ => Spec.v_var x
-    | v_tt => Spec.v_tt
-    | v_fst v => Spec.v_fst (undec v)
-    | v_snd v => Spec.v_snd (undec v)
-    | v_fanout v v' => Spec.v_fanout (undec v) (undec v')
-    end.
-
-  Lemma wf {Γ t} (v: term Γ t): Γ ⊢ undec v in t.
-  Proof.
-    induction v.
-    all: cbn.
-    all: econstructor.
-    all: eauto.
-    apply find_sound.
-    auto.
-  Qed.
-
-  Lemma wf_undec_dec {Γ v t} (p: typecheck Γ v = Some t): Γ ⊢ undec (dec t v p) in t.
-  Proof.
-    apply wf.
-  Qed.
-
-  Lemma undec_dec {Γ v}:
-    if dec' Γ v is Some (existT _ _ v')
-    then
-      undec v' = v
-    else
-      True.
-  Proof.
-    induction v.
-    all: cbn.
-    - destruct find_dec eqn:q.
-      2: auto.
-      cbn.
-      auto.
-    - auto.
-    - destruct (dec' Γ v).
-      2: auto.
-      destruct s.
-      destruct x.
-      1: auto.
-      cbn.
-      rewrite IHv.
-      auto.
-    - destruct (dec' Γ v).
-      2: auto.
-      destruct s.
-      destruct x.
-      1: auto.
-      cbn.
-      rewrite IHv.
-      auto.
-    - destruct (dec' Γ v1).
-      2: auto.
-      destruct s.
-      destruct (dec' Γ v2).
-      2: auto.
-      destruct s.
-      cbn.
-      rewrite IHv1, IHv2.
-      auto.
-  Qed.
-End Dec.
-
-Section Cartesian.
-  Import CategoryNotations.
-
-  Context {C: Category}.
-
-  Context {unit: C}.
-  Context {prod: C → C → C}.
-
-  Context {bang: ∀ c, C c unit}.
-  Context {fst: ∀ a b, C (prod a b) a}.
-  Context {snd: ∀ a b, C (prod a b) b}.
-  Context {fanout: ∀ a b c, C c a → C c b → C c (prod a b)}.
-
-  Fixpoint obj t: C :=
-    match t with
-    | t_unit => unit
-    | t_prod t t' => prod (obj t) (obj t')
-    end.
-
-  Fixpoint env Γ: C :=
-    if Γ is cons ((_, t)) T
-    then
-      prod (obj t) (env T)
-    else
-      unit.
-
-  Open Scope category.
-
-  Import Dec.
-
-  Fixpoint mor' {Γ t} (v: Dec.term Γ t) {A} {struct v}: (∀ x t, find x Γ = Some t → C A (obj t)) → C A (obj t) :=
-    match v in term _ t' return (∀ x t, find x Γ = Some t → C A (obj t)) → C A (obj t') with
-    | @v_var _ t' x p => λ h, h x t' p
-    | v_tt => λ _, bang _
-    | v_fst v => λ h, compose (fst _ _) (mor' v h)
-    | v_snd v => λ h, compose (snd _ _) (mor' v h)
-    | v_fanout v v' => λ h, fanout _ _ _ (mor' v h) (mor' v' h)
-    end.
-
-  Program Fixpoint find x t Γ (p: Environment.find x Γ = Some t): C (env Γ) (obj t) :=
-    match Γ with
-    | cons (y, t') T =>
-        match eq_var x y with
-        | left _ =>
-            fst (obj t) (env T)
-        | right _ =>
-            compose (find x t T _) (snd (obj t') (env T))
-        end
-    | nil => match _: False with end
-    end %list.
-
-  Next Obligation.
-  Proof.
-    cbn in p.
-    destruct eq_var in p.
-    2: contradiction.
-    inversion p.
+    all: intros t' q.
+    all: inversion q.
     all: subst.
-    all: auto.
-  Qed.
-
-  Definition mor {Γ t} v (p: typecheck Γ v = Some t) := mor' (Dec.dec t v p) (λ x t, find _ _ _).
-End Cartesian.
+    all: try (econstructor; eauto).
+  - intros Γ V' t x p V.
+    destruct V.
+    all: cbn.
+    all: intros t' q.
+    all: inversion q.
+    all: subst.
+    all: try (econstructor; eauto).
+    destruct eq_var.
+    + subst.
+      inversion H1.
+      2: contradiction.
+      subst.
+      auto.
+    + inversion H1.
+      1: contradiction.
+      subst.
+      constructor.
+      auto.
+Qed.
